{
"cells": [
{"cell_type":    "code", "execution_count":null, "metadata":{}, "source":["%%html\n<link href=\"http://mathbook.pugetsound.edu/beta/mathbook-content.css\" rel=\"stylesheet\" type=\"text/css\" />\n<link href=\"https://aimath.org/mathbook/mathbook-add-on.css\" rel=\"stylesheet\" type=\"text/css\" />\n<style>.subtitle {font-size:medium; display:block}</style>\n<link href=\"https://fonts.googleapis.com/css?family=Open+Sans:400,400italic,600,600italic\" rel=\"stylesheet\" type=\"text/css\" />\n<link href=\"https://fonts.googleapis.com/css?family=Inconsolata:400,700&subset=latin,latin-ext\" rel=\"stylesheet\" type=\"text/css\" /><!-- Hide this cell. -->\n<script>\nvar cell = $(\".container .cell\").eq(0), ia = cell.find(\".input_area\")\nif (cell.find(\".toggle-button\").length == 0) {\nia.after(\n    $('<button class=\"toggle-button\">Toggle hidden code</button>').click(\n        function (){ ia.toggle() }\n        )\n    )\nia.hide()\n}\n</script>\n"], "outputs":[]},
{"cell_type":"markdown", "metadata":{}, "source":["**Important:** to view this notebook properly you will need to execute the cell above, which assumes you have an Internet connection.  It should already be selected, or place your cursor anywhere above to select.  Then press the \"Run\" button in the menu bar above (the right-pointing arrowhead), or press Shift-Enter on your keyboard."]},
{"cell_type":"markdown", "metadata":{}, "source":["$\n\\newcommand{\\lt}{<}\n\\newcommand{\\gt}{>}\n\\newcommand{\\amp}{&}\n$"]},
{"cell_type":"markdown", "metadata":{}, "source":["<div class=\"mathbook-content\"></div>"]},
{"cell_type":"markdown", "metadata":{}, "source":["<div class=\"mathbook-content\"><h1 class=\"heading\"><span class=\"title\">Differential Equations Worksheet</span><span class=\"subtitle\">Accompanies Section 1.5 in ODEP</span></h1><div class=\"author\"><div class=\"author-name\">Dave Rosoff</div><div class=\"author-info\">Department of Mathematics and Physical Sciences<br />The College of Idaho</div></div><time class=\"date\">Spring 2018</time></div>"]},
{"cell_type":"markdown", "metadata":{}, "source":["<div class=\"mathbook-content\"><h2 class=\"heading hide-type\" alt=\"Section 1 First-order linear differential equations\"><span class=\"type\">Section</span><span class=\"codenumber\">1</span><span class=\"title\">First-order linear differential equations</span></h2></div>"]},
{"cell_type":"markdown", "metadata":{}, "source":["<div class=\"mathbook-content\"><p id=\"p-1\">In this workshop, you will see how to solve (remember the technical meaning of this word) linear first-order differential equations, that is, equations of the form</p><div class=\"displaymath\">\n\\begin{equation*}\n\\frac{dy}{dt} + p(t)y = g(t)\\text{.}\n\\end{equation*}\n</div></div>"]},
{"cell_type":"markdown", "metadata":{}, "source":["<div class=\"mathbook-content\"><article class=\"example-like\" id=\"activity-integrating-factors-1\"><h6 class=\"heading\"><span class=\"type\">Activity</span><span class=\"codenumber\">1.1</span><span class=\"title\">Integrating factors</span></h6><article class=\"exercise-like\" id=\"task-mult-by-mu\"><h6 class=\"heading\"><span class=\"codenumber\">(a)</span></h6><p id=\"p-4\">Multiply this equation by a new unknown function $\\mu(t)\\text{.}$</p><div class=\"solutions\"><span class=\"solution\"><a knowl=\"\" class=\"id-ref\" refid=\"hk-answer-mult-by-mu\" id=\"answer-mult-by-mu\"><span class=\"type\">Answer</span></a></span><div id=\"hk-answer-mult-by-mu\" class=\"hidden-content tex2jax_ignore\"><span class=\"solution\"><div class=\"displaymath\" id=\"p-5\">\n\\begin{equation*}\n\\mu(t) \\frac{dy}{dt} + \\mu(t) \\frac{y(t)}{2} = \\frac{1}{2} \\mu(t) e^{t/3}\\text{.}\n\\end{equation*}\n</div></span></div></div></article><article class=\"exercise-like\" id=\"task-apply-product-rule\"><h6 class=\"heading\"><span class=\"codenumber\">(b)</span></h6><p id=\"p-6\">According to the product rule, what is $(\\mu(t)y(t))'\\text{?}$</p><div class=\"displaymath\">\n\\begin{equation*}\n\\frac{d}{dt}\\left(\\mu(t) y\\right) = \\underline{\\hspace{18.1818181818182em}}\n\\end{equation*}\n</div><div class=\"solutions\"><span class=\"solution\"><a knowl=\"\" class=\"id-ref\" refid=\"hk-answer-apply-product-rule\" id=\"answer-apply-product-rule\"><span class=\"type\">Answer</span></a></span><div id=\"hk-answer-apply-product-rule\" class=\"hidden-content tex2jax_ignore\"><span class=\"solution\"><div class=\"displaymath\" id=\"p-7\">\n\\begin{equation*}\n\\frac{d}{dt}(\\mu(t) y(t)) = \\frac{d\\mu}{dt} y(t) + \\mu(t) \\frac{dy}{dt}\\text{.}\n\\end{equation*}\n</div></span></div></div></article><article class=\"exercise-like\" id=\"task-new-equation\"><h6 class=\"heading\"><span class=\"codenumber\">(c)</span></h6><p id=\"p-8\">Observe that the expression $\\mu(t) dy/dt$ appears in both of the equations you found in <a href=\"LFO.ipynb#task-mult-by-mu\" class=\"xref\" alt=\"Task 1.1.a \" title=\"Task 1.1.a \">Task a</a> and <a href=\"LFO.ipynb#task-apply-product-rule\" class=\"xref\" alt=\"Task 1.1.b \" title=\"Task 1.1.b \">Task b</a>.</p><div class=\"solutions\"><span class=\"solution\"><a knowl=\"\" class=\"id-ref\" refid=\"hk-answer-3\" id=\"answer-3\"><span class=\"type\">Answer</span></a></span><div id=\"hk-answer-3\" class=\"hidden-content tex2jax_ignore\"><span class=\"solution\"><p id=\"p-9\">Indeed, it does. See <a href=\"LFO.ipynb#answer-mult-by-mu\" class=\"xref\" alt=\"Answer 1.1.a.1 \" title=\"Answer 1.1.a.1 \">Answer 1 of Task 1.1.a</a> and <a href=\"LFO.ipynb#answer-apply-product-rule\" class=\"xref\" alt=\"Answer 1.1.b.1 \" title=\"Answer 1.1.b.1 \">Answer 1 of Task 1.1.b</a>.</p></span></div></div></article><article class=\"exercise-like\" id=\"task-equate-two-sides\"><h6 class=\"heading\"><span class=\"codenumber\">(d)</span></h6><p id=\"p-10\">Write down an equation that asserts the equality of the equation sides containing $\\mu(t) dy/dt\\text{.}$</p><div class=\"solutions\"><span class=\"solution\"><a knowl=\"\" class=\"id-ref\" refid=\"hk-answer-4\" id=\"answer-4\"><span class=\"type\">Answer</span></a></span><div id=\"hk-answer-4\" class=\"hidden-content tex2jax_ignore\"><span class=\"solution\"><div class=\"displaymath\" id=\"p-11\">\n\\begin{equation*}\n\\mu(t) \\frac{dy}{dt} + \\mu(t) \\frac{y(t)}{2} = \\frac{d\\mu}{dt} y(t) + \\mu(t) \\frac{dy}{dt} \\text{.}\n\\end{equation*}\n</div></span></div></div></article><article class=\"exercise-like\" id=\"task-find-mu\"><h6 class=\"heading\"><span class=\"codenumber\">(e)</span></h6><p id=\"p-12\">Simplify the equation you found in <a href=\"LFO.ipynb#task-equate-two-sides\" class=\"xref\" alt=\"Task 1.1.d \" title=\"Task 1.1.d \">Task d</a>, isolate $d\\mu/dt\\text{,}$ and integrate to find an expression for $\\mu(t)\\text{.}$ (Choose the simplest value for the constant of integration.)</p><div class=\"solutions\"><span class=\"solution\"><a knowl=\"\" class=\"id-ref\" refid=\"hk-answer-5\" id=\"answer-5\"><span class=\"type\">Answer</span></a></span><div id=\"hk-answer-5\" class=\"hidden-content tex2jax_ignore\"><span class=\"solution\"><div class=\"displaymath\" id=\"p-13\">\n\\begin{equation*}\n\\mu(t) = e^{t/2}\\text{.}\n\\end{equation*}\n</div></span></div></div></article><article class=\"exercise-like\" id=\"task-substitute-mu\"><h6 class=\"heading\"><span class=\"codenumber\">(f)</span></h6><p id=\"p-14\">Now that your <dfn class=\"terminology\">integrating factor</dfn> $\\mu(t)$ is in hand, substitute it into the equation you found in <a href=\"LFO.ipynb#task-new-equation\" class=\"xref\" alt=\"Task 1.1.c \" title=\"Task 1.1.c \">Task c</a>.</p><div class=\"solutions\"><span class=\"solution\"><a knowl=\"\" class=\"id-ref\" refid=\"hk-answer-6\" id=\"answer-6\"><span class=\"type\">Answer</span></a></span><div id=\"hk-answer-6\" class=\"hidden-content tex2jax_ignore\"><span class=\"solution\"><div class=\"displaymath\" id=\"p-15\">\n\\begin{align*}\ne^{t/2} \\frac{dy}{dt} + e^{t/2} \\frac{y(t)}{2} \\amp = \\frac{1}{2} e^{t/2} e^{t/3}\\\\\n\\amp = \\frac{1}{2} e^{5/6}\\text{.}\n\\end{align*}\n</div></span></div></div></article><article class=\"exercise-like\" id=\"task-recognize-derivative\"><h6 class=\"heading\"><span class=\"codenumber\">(g)</span></h6><p id=\"p-16\">Apply the result of <a href=\"LFO.ipynb#task-apply-product-rule\" class=\"xref\" alt=\"Task 1.1.b \" title=\"Task 1.1.b \">Task b</a> to the equation you found in <a href=\"LFO.ipynb#task-substitute-mu\" class=\"xref\" alt=\"Task 1.1.f \" title=\"Task 1.1.f \">Task f</a>.</p><div class=\"solutions\"><span class=\"solution\"><a knowl=\"\" class=\"id-ref\" refid=\"hk-answer-7\" id=\"answer-7\"><span class=\"type\">Answer</span></a></span><div id=\"hk-answer-7\" class=\"hidden-content tex2jax_ignore\"><span class=\"solution\"><div class=\"displaymath\" id=\"p-17\">\n\\begin{equation*}\n\\frac{d}{dt} \\left( e^{t/2} y(t) \\right) = \\frac{1}{2} e^{5t/6}\n\\end{equation*}\n</div></span></div></div></article><article class=\"exercise-like\" id=\"task-use-ftc\"><h6 class=\"heading\"><span class=\"codenumber\">(h)</span></h6><p id=\"p-18\">Integrate, using the Fundamental Theorem of Calculus on both sides.</p><div class=\"solutions\"><span class=\"solution\"><a knowl=\"\" class=\"id-ref\" refid=\"hk-answer-8\" id=\"answer-8\"><span class=\"type\">Answer</span></a></span><div id=\"hk-answer-8\" class=\"hidden-content tex2jax_ignore\"><span class=\"solution\"><div class=\"displaymath\" id=\"p-19\">\n\\begin{align*}\ne^{t/2} y(t) \\amp = \\frac{1}{2} \\frac{6}{5} e^{5t/6} + C\\\\\n\\amp = \\frac{3}{5} e^{5t/6} + C\n\\end{align*}\n</div></span></div></div></article><article class=\"exercise-like\" id=\"task-finish-solve\"><h6 class=\"heading\"><span class=\"codenumber\">(i)</span></h6><p id=\"p-20\">Solve the equation you found in <a href=\"LFO.ipynb#task-use-ftc\" class=\"xref\" alt=\"Task 1.1.h \" title=\"Task 1.1.h \">Task h</a> for $y(t)\\text{.}$</p><div class=\"solutions\"><span class=\"solution\"><a knowl=\"\" class=\"id-ref\" refid=\"hk-answer-9\" id=\"answer-9\"><span class=\"type\">Answer</span></a></span><div id=\"hk-answer-9\" class=\"hidden-content tex2jax_ignore\"><span class=\"solution\"><div class=\"displaymath\" id=\"p-21\">\n\\begin{equation*}\ny(t) = \\frac{3}{5} e^{t/3} + Ce^{-t/2}\\text{.}\n\\end{equation*}\n</div></span></div></div></article><article class=\"exercise-like\" id=\"task-check\"><h6 class=\"heading\"><span class=\"codenumber\">(j)</span></h6><p id=\"p-22\">Check that $y(t)$ as found in <a href=\"LFO.ipynb#task-finish-solve\" class=\"xref\" alt=\"Task 1.1.i \" title=\"Task 1.1.i \">Task i</a> is really a solution to the original <a href=\"LFO.ipynb#mjx-eqn-eq-linear-1\" class=\"xref\" alt=\"Equation 1.1 \" title=\"Equation 1.1 \">(1.1)</a>.</p><div class=\"solutions\"><span class=\"solution\"><a knowl=\"\" class=\"id-ref\" refid=\"hk-solution-1\" id=\"solution-1\"><span class=\"type\">Solution</span></a></span><div id=\"hk-solution-1\" class=\"hidden-content tex2jax_ignore\"><span class=\"solution\"><p id=\"p-23\">Since $y = \\frac{3}{5} e^{t/3} + Ce^{-t/2}\\text{,}$ we can differentiate to find</p><div class=\"displaymath\">\n\\begin{equation*}\ny' = \\frac{1}{5} e^{t/3} - \\frac{1}{2} Ce^{-t/2}\\text{.}\n\\end{equation*}\n</div><p>Substitution into <a href=\"LFO.ipynb#mjx-eqn-eq-linear-1\" class=\"xref\" alt=\"Equation 1.1 \" title=\"Equation 1.1 \">(1.1)</a> then gives</p><div class=\"displaymath\">\n\\begin{align*}\n\\frac{dy}{dt} + \\frac{y(t)}{2} \\amp = \\frac{1}{5} e^{t/3} - \\frac{1}{2} Ce^{-t/2} + \\frac{3}{10} e^{t/3} + \\frac{1}{2} Ce^{-t/2}\\\\\n\\amp = \\frac{1}{2} e^{t/3}\\text{,}\n\\end{align*}\n</div><p>as required.</p></span></div></div></article></article></div>"]},
{"cell_type":"markdown", "metadata":{}, "source":["<div class=\"mathbook-content\"><article class=\"example-like\" id=\"activity-practice-integrating-factors\"><h6 class=\"heading\"><span class=\"type\">Activity</span><span class=\"codenumber\">1.3</span><span class=\"title\">Practice integrating factors</span></h6><article class=\"exercise-like\" id=\"task-practice-mult-by-mu\"><h6 class=\"heading\"><span class=\"codenumber\">(a)</span></h6><p id=\"p-25\">Multiply both sides by $\\mu(t)\\text{.}$</p></article><article class=\"exercise-like\" id=\"task-practice-apply-product-rule\"><h6 class=\"heading\"><span class=\"codenumber\">(b)</span></h6><p id=\"p-26\">Recall what the product rule tells you about $(\\mu(t) y(t))'\\text{.}$</p></article><article class=\"exercise-like\" id=\"task-practice-equate-two-sides\"><h6 class=\"heading\"><span class=\"codenumber\">(c)</span></h6><p id=\"p-27\">Write an equation asserting the equality of two different expressions involving $\\mu(t) dy/dt\\text{.}$</p></article><article class=\"exercise-like\" id=\"task-practice-find-mu\"><h6 class=\"heading\"><span class=\"codenumber\">(d)</span></h6><p id=\"p-28\">Solve your equation for the integrating factor $\\mu(t)\\text{.}$</p><div class=\"solutions\"><span class=\"solution\"><a knowl=\"\" class=\"id-ref\" refid=\"hk-hint-1\" id=\"hint-1\"><span class=\"type\">Hint</span></a></span><div id=\"hk-hint-1\" class=\"hidden-content tex2jax_ignore\"><span class=\"solution\"><p id=\"p-29\">Remember, at this stage we can choose any convenient constant of integration: all the possible functions $\\mu(t)$ are equally good.</p></span></div></div></article><article class=\"exercise-like\" id=\"task-practice-finish-solve\"><h6 class=\"heading\"><span class=\"codenumber\">(e)</span></h6><p id=\"p-30\">Use $\\mu(t)$ and one more integration to solve <a href=\"LFO.ipynb#mjx-eqn-eq-linear-2\" class=\"xref\" alt=\"Equation 1.2 \" title=\"Equation 1.2 \">(1.2)</a>.</p><div class=\"solutions\"><span class=\"solution\"><a knowl=\"\" class=\"id-ref\" refid=\"hk-hint-2\" id=\"hint-2\"><span class=\"type\">Hint</span></a></span><div id=\"hk-hint-2\" class=\"hidden-content tex2jax_ignore\"><span class=\"solution\"><p id=\"p-31\">Here, the constant of integration is essential. We want to know all of the (infinitely many) functions that satisfy <a href=\"LFO.ipynb#mjx-eqn-eq-linear-2\" class=\"xref\" alt=\"Equation 1.2 \" title=\"Equation 1.2 \">(1.2)</a>, not just one of them.</p></span></div></div></article><article class=\"exercise-like\" id=\"task-practice-check\"><h6 class=\"heading\"><span class=\"codenumber\">(f)</span></h6><p id=\"p-32\">Differentiate the function you found in <a href=\"LFO.ipynb#task-practice-finish-solve\" class=\"xref\" alt=\"Task 1.3.e \" title=\"Task 1.3.e \">Task e</a> and substitute into <a href=\"LFO.ipynb#mjx-eqn-eq-linear-2\" class=\"xref\" alt=\"Equation 1.2 \" title=\"Equation 1.2 \">(1.2)</a> to verify that your solution is correct.</p></article></article></div>"]},
{"cell_type":"markdown", "metadata":{}, "source":["<div class=\"mathbook-content\"><p id=\"p-33\">The foregoing activities should illustrate the general principle. In ODEP Section 1.5.2 we see that, to solve the equation</p><div class=\"displaymath\">\n\\begin{equation}\ny' + p(t)y = q(t)\\text{,}\\label{eq-linear-general}\\tag{1.3}\n\\end{equation}\n</div><p>we can always choose $\\mu(t) = \\underline{\\hspace{18.1818181818182em}}\\text{,}$ where $P(t)$ is any antiderivative of $p(t)\\text{.}$</p></div>"]},
{"cell_type":"markdown", "metadata":{}, "source":["<div class=\"mathbook-content\"><article class=\"remark-like\" id=\"warning-1\"><h6 class=\"heading\"><span class=\"type\">Warning</span><span class=\"codenumber\">1</span></h6><p id=\"p-34\">Note that the formula for the integrating factor assumes that the differential equation has been put into a certain <dfn class=\"terminology\">standard form</dfn>. If you memorize the former, be sure to remember the latter as well!</p></article></div>"]}
],
"nbformat": 4, "nbformat_minor": 0, "metadata": {"kernelspec": {"display_name": "", "name": "sagemath"}, "language_info": {"codemirror_mode": {"name": "ipython", "version": 2}, "file_extension": ".py", "mimetype": "text/x-python", "name": "python", "nbconvert_exporter": "python", "pygments_lexer": "ipython2", "version": "2.7.8"}, "name": "LFO.ipynb"}
}